src/cbor/CBOR.SteelST.fsti
@@ -213,6 +213,66 @@ val read_cbor
     (SZ.v sz == Seq.length va \/ SZ.v sz == A.length a)
     (fun _ -> True)
 
+noextract
+let read_deterministically_encoded_cbor_success_postcond
+  (va: Ghost.erased (Seq.seq U8.t))
+  (c: read_cbor_success_t)
+  (v: Cbor.raw_data_item)
+  (rem: Seq.seq U8.t)
+: Tot prop
+= read_cbor_success_postcond va c v rem /\
+  Cbor.data_item_wf Cbor.deterministically_encoded_cbor_map_key_order v == true
+
+[@@__reduce__]
+let read_deterministically_encoded_cbor_success_post
+  (a: A.array U8.t)
+  (p: perm)
+  (va: Ghost.erased (Seq.seq U8.t))
+  (c: read_cbor_success_t)
+: Tot vprop
+= exists_ (fun v -> exists_ (fun rem ->
+    raw_data_item_match c.read_cbor_payload v `star`
+    A.pts_to c.read_cbor_remainder p rem `star`
+    ((raw_data_item_match c.read_cbor_payload v `star` A.pts_to c.read_cbor_remainder p rem) `implies_`
+      A.pts_to a p va) `star`
+    pure (read_deterministically_encoded_cbor_success_postcond va c v rem)
+  ))
+
+noextract
+let read_deterministically_encoded_cbor_error_postcond
+  (va: Ghost.erased (Seq.seq U8.t))
+: Tot prop
+= forall v . Cbor.serialize_cbor v == Seq.slice va 0 (min (Seq.length (Cbor.serialize_cbor v)) (Seq.length va)) ==> Cbor.data_item_wf Cbor.deterministically_encoded_cbor_map_key_order v == false
+
+[@@__reduce__]
+let read_deterministically_encoded_cbor_error_post
+  (a: A.array U8.t)
+  (p: perm)
+  (va: Ghost.erased (Seq.seq U8.t))
+: Tot vprop
+= A.pts_to a p va `star` pure (read_deterministically_encoded_cbor_error_postcond va)
+
+let read_deterministically_encoded_cbor_post
+  (a: A.array U8.t)
+  (p: perm)
+  (va: Ghost.erased (Seq.seq U8.t))
+  (res: read_cbor_t)
+: Tot vprop
+= match res with
+  | ParseError -> read_deterministically_encoded_cbor_error_post a p va
+  | ParseSuccess c -> read_deterministically_encoded_cbor_success_post a p va c
+
+val read_deterministically_encoded_cbor
+  (#va: Ghost.erased (Seq.seq U8.t))
+  (#p: perm)
+  (a: A.array U8.t)
+  (sz: SZ.t)
+: ST read_cbor_t
+    (A.pts_to a p va)
+    (fun res -> read_deterministically_encoded_cbor_post a p va res)
+    (SZ.v sz == Seq.length va \/ SZ.v sz == A.length a)
+    (fun _ -> True)
+
 (* Destructors and constructors *)
 
 val destr_cbor_int64
